start work on implementing fa2 contract

execution/theories/Examples/FA2Token.v
@@ -8,15 +8,98 @@ From RecordUpdate Require Import RecordUpdate.
 From Coq Require Import List.
 Require Import Serializable.
 Require Import Blockchain.
-Require Import FA2Interface. 
 Import ListNotations.
 Import RecordSetNotations.
 
 Section FA2Token.
-Print FA2Interface.
 Context {BaseTypes : ChainBase}.
+Require Import FA2Interface. 
 Set Primitive Projections.
 Set Nonrecursive Elimination Schemes.
+Open Scope N_scope.
+
+Inductive Msg := 
+  | msg_transfer : list transfer -> Msg
+  | msg_balance_of : balance_of_param -> Msg
+  | msg_total_supply : total_supply_param -> Msg
+  | msg_token_metadata : token_metadata_param -> Msg
+  | msg_permissions_descriptor : permissions_descriptor -> Msg (* TODO fix callback type *)
+  | msg_update_operators : list update_operator -> Msg
+  | msg_is_operator : is_operator_param -> Msg.
+
+Record TokenLedger := 
+  build_token_ledger {
+    fungible : bool;
+    balances : FMap Address N
+}.
+
+Record State :=
+  build_state {
+    assets: FMap token_id TokenLedger 
+  }.
+
+Record Setup :=
+  build_setup {
+    setup_total_supply : list (token_id * N);
+  }.
+
+Instance token_ledger_settable : Settable _ :=
+  settable! build_token_ledger <fungible; balances>.
+Instance state_settable : Settable _ :=
+  settable! build_state <assets>.
+Instance setup_settable : Settable _ :=
+  settable! build_setup <setup_total_supply>.
+
+Section Serialization.
+
+Global Instance setup_serializable : Serializable Setup :=
+  Derive Serializable Setup_rect <build_setup>.
+
+Global Instance msg_serializable : Serializable Msg :=
+  Derive Serializable Msg_rect <msg_transfer, msg_balance_of, msg_total_supply, msg_token_metadata, msg_permissions_descriptor, msg_update_operators, msg_is_operator>.
+
+Global Instance TokenLedger_serializable : Serializable TokenLedger :=
+  Derive Serializable TokenLedger_rect <build_token_ledger>.
+
+Global Instance state_serializable : Serializable State :=
+	Derive Serializable State_rect <build_state>.
+	
+End Serialization.
+
+Definition returnIf (cond : bool) := if cond then None else Some tt.
+
+Definition address_has_sufficient_asset_balance (token_id : token_id) 
+                                                (owner : Address) 
+                                                (transaction_amount : N) 
+                                                (state : State) 
+                                                : option unit :=
+  do ledger <- FMap.find token_id state.(assets) ;
+  do owner_balance <- FMap.find owner ledger.(balances) ;
+  if transaction_amount <=? owner_balance
+  then Some tt
+  else None. 
+
+(* TODO: dummy implementation for now - only owner has permission to transfer token*)
+Definition address_has_transfer_permission (caller owner : Address) : option unit := 
+  if address_eqb caller owner then Some tt else None.
 
 
+Definition address_balance (token_id : token_id)
+                           (addr : Address)
+                           (state : State) : option N := 
+  do ledger <- FMap.find token_id state.(assets) ;
+  FMap.find addr ledger.(balances).
+
+Definition try_transfer (caller : Address)
+                        (params : transfer)
+                        (state : State)
+                        : option TokenLedger :=
+  (* do _ <- address_has_sufficient_asset_balance transfer_params.(transfer_token_id) transfer_params.(from_) transfer_params.(amount) ; *)
+  do _ <- address_has_transfer_permission caller params.(from_) ;
+  do ledger <- FMap.find params.(transfer_token_id) state.(assets) ;
+  do current_owner_balance <- address_balance params.(transfer_token_id) params.(from_) state ;
+  let new_balances : FMap Address N := FMap.add params.(from_) (current_owner_balance - params.(amount)) ledger.(balances) in
+  let new_balances : FMap Address N := FMap.partial_alter (fun balance => Some ((with_default 0 balance) + params.(amount))) params.(to_) new_balances in
+  Some (ledger<|balances := new_balances|>).
+  
 End FA2Token.
